examples/unit-tests/utils.fst
@@ -22,7 +22,7 @@ assume In_tl: forall 'a (hd:'a) (x:'a) (tl:list 'a). In x tl ==> In x (Cons hd t
 (* assume NotinNil: forall 'a (x:'a). not (In x Nil) *)
 (* assume NotinCons: forall 'a (x:'a) (y:'a) (tl:list 'a). not(In x tl) /\ x<>y ==> not(In x (Cons y tl)) *)
 
-val mem: x:'a -> l:list 'a -> b:bool{b=true <==> In x l}
+val mem: x:'a -> l:list 'a -> b:bool{b==true <==> In x l}
 let rec mem x = function
   | [] -> false
   | hd::tl -> if hd = x then true else mem x tl
@@ -52,7 +52,7 @@ let rec assoc a x = match x with
   | [] -> None
   | (a', b)::tl -> if a=a' then Some b else assoc a tl
 
-val append: x:list 'a -> y:list 'a -> z:list 'a { forall (a:'a). In a z <==> In a x \/ In a y }
+val append: x:list 'a -> y:list 'a -> z:list 'a { forall a. In a z <==> In a x \/ In a y }
 let rec append x y = match x with
   | [] -> y
   | a::tl -> a::append tl y
